libcrux-ml-kem/proofs/fstar/extraction/Libcrux_ml_kem.Polynomial.fst
@@ -205,8 +205,6 @@ let from_bytes
   in
   result
 
-#push-options "--admit_smt_queries true"
-
 let to_bytes
       (#v_Vector: Type0)
       (#[FStar.Tactics.Typeclasses.tcresolve ()]
@@ -253,10 +251,6 @@ let to_bytes
   in
   out
 
-#pop-options
-
-#push-options "--admit_smt_queries true"
-
 let add_to_ring_element
       (#v_Vector: Type0)
       (v_K: usize)
@@ -265,38 +259,50 @@ let add_to_ring_element
           Libcrux_ml_kem.Vector.Traits.t_Operations v_Vector)
       (myself rhs: t_PolynomialRingElement v_Vector)
      =
+  let e_myself:t_Array v_Vector (mk_usize 16) = myself.f_coefficients in
   let myself:t_PolynomialRingElement v_Vector =
     Rust_primitives.Hax.Folds.fold_range (mk_usize 0)
       (Core.Slice.impl__len #v_Vector (myself.f_coefficients <: t_Slice v_Vector) <: usize)
-      (fun myself temp_1_ ->
+      (fun myself i ->
           let myself:t_PolynomialRingElement v_Vector = myself in
-          let _:usize = temp_1_ in
-          true)
+          let i:usize = i in
+          v i <= v v_VECTORS_IN_RING_ELEMENT /\
+          (forall (j: nat).
+              (j >= v i /\ j < v v_VECTORS_IN_RING_ELEMENT) ==>
+              (let _myself_j = i1.f_to_i16_array (e_myself.[ sz j ]) in
+                let myself_j = i1.f_to_i16_array (myself.f_coefficients.[ sz j ]) in
+                let rhs_j = i1.f_to_i16_array (rhs.f_coefficients.[ sz j ]) in
+                myself_j == _myself_j /\ Libcrux_ml_kem.Vector.Traits.Spec.add_pre myself_j rhs_j)) /\
+          (forall (j: nat).
+              j < v i ==>
+              (let _myself_j = i1.f_to_i16_array (e_myself.[ sz j ]) in
+                let myself_j = i1.f_to_i16_array (myself.f_coefficients.[ sz j ]) in
+                let rhs_j = i1.f_to_i16_array (rhs.f_coefficients.[ sz j ]) in
+                Libcrux_ml_kem.Vector.Traits.Spec.add_post _myself_j rhs_j myself_j)))
       myself
       (fun myself i ->
           let myself:t_PolynomialRingElement v_Vector = myself in
           let i:usize = i in
-          {
-            myself with
-            f_coefficients
-            =
-            Rust_primitives.Hax.Monomorphized_update_at.update_at_usize myself.f_coefficients
-              i
-              (Libcrux_ml_kem.Vector.Traits.f_add #v_Vector
-                  #FStar.Tactics.Typeclasses.solve
-                  (myself.f_coefficients.[ i ] <: v_Vector)
-                  (rhs.f_coefficients.[ i ] <: v_Vector)
-                <:
-                v_Vector)
+          let myself:t_PolynomialRingElement v_Vector =
+            {
+              myself with
+              f_coefficients
+              =
+              Rust_primitives.Hax.Monomorphized_update_at.update_at_usize myself.f_coefficients
+                i
+                (Libcrux_ml_kem.Vector.Traits.f_add #v_Vector
+                    #FStar.Tactics.Typeclasses.solve
+                    (myself.f_coefficients.[ i ] <: v_Vector)
+                    (rhs.f_coefficients.[ i ] <: v_Vector)
+                  <:
+                  v_Vector)
+            }
             <:
-            t_Array v_Vector (mk_usize 16)
-          }
-          <:
-          t_PolynomialRingElement v_Vector)
+            t_PolynomialRingElement v_Vector
+          in
+          myself)
   in
   myself
-
-#pop-options
 
 #push-options "--admit_smt_queries true"
 
@@ -641,17 +647,6 @@ let impl_2__ZERO
   <:
   t_PolynomialRingElement v_Vector
 
-let impl_2__add_to_ring_element
-      (#v_Vector: Type0)
-      (v_K: usize)
-      (#[FStar.Tactics.Typeclasses.tcresolve ()]
-          i1:
-          Libcrux_ml_kem.Vector.Traits.t_Operations v_Vector)
-      (self rhs: t_PolynomialRingElement v_Vector)
-     =
-  let self:t_PolynomialRingElement v_Vector = add_to_ring_element #v_Vector v_K self rhs in
-  self
-
 let impl_2__poly_barrett_reduce
       (#v_Vector: Type0)
       (#[FStar.Tactics.Typeclasses.tcresolve ()]
@@ -839,3 +834,14 @@ let vec_to_bytes
           out)
   in
   out
+
+let impl_2__add_to_ring_element
+      (#v_Vector: Type0)
+      (v_K: usize)
+      (#[FStar.Tactics.Typeclasses.tcresolve ()]
+          i1:
+          Libcrux_ml_kem.Vector.Traits.t_Operations v_Vector)
+      (self rhs: t_PolynomialRingElement v_Vector)
+     =
+  let self:t_PolynomialRingElement v_Vector = add_to_ring_element #v_Vector v_K self rhs in
+  self
