libcrux-ml-kem/proofs/fstar/extraction/Libcrux_ml_kem.Vector.Traits.Spec.fst
@@ -1,0 +1,10 @@
+module Libcrux_ml_kem.Vector.Traits.Spec
+#set-options "--fuel 0 --ifuel 1 --z3rlimit 80"
+open Core
+open FStar.Mul
+
+let add_pre (lhs rhs: t_Array i16 (mk_usize 16)) : Hax_lib.Prop.t_Prop =
+  forall i. i < 16 ==> Spec.Utils.is_intb (pow2 15 - 1) (v (Seq.index lhs i) + v (Seq.index rhs i))
+
+let add_post (lhs rhs result: t_Array i16 (mk_usize 16)) : Hax_lib.Prop.t_Prop =
+  forall i. i < 16 ==> (v (Seq.index result i) == v (Seq.index lhs i) + v (Seq.index rhs i))
